[sledge sem] Update LLVM and LLAIR sem for consistent stuckness
Summary:
Previously, the LLVM semantics could be stuck where the LLAIR semantics
was not yet stuck, but would become stuck (at the same place) after
taking a step. This was due to LLVM using the traditional definition of
stuck states: any state from which there are no transitions. However,
LLAIR cannot do that because it might get stuck in the middle of a block
that contains several visible stores. We don't want to consider the
whole block stuck, nor can we finish it. Thus, the LLAIR definition of
stuckness is when the state has the stuck flag set which happens when
stopping in the middle of a block after encountering a stuck
instruction. Now LLVM takes the same approach.

Reviewed By: jberdine

Differential Revision: D17855085

fbshipit-source-id: a094d25d5

sledge/semantics/llairScript.sml
@@ -433,7 +433,7 @@ Inductive step_term:
    Lab_name fname bname = (case alookup table idx of Some lab => lab | None => default)
    ⇒
    step_term prog s
-     (Switch e table default)
+     (Switch e table default) Tau
      (s with bp := Lab_name fname bname)) ∧
 
   (∀prog s e labs i idx idx_size.
@@ -441,7 +441,7 @@ Inductive step_term:
    idx < length labs
    ⇒
    step_term prog s
-     (Iswitch e labs)
+     (Iswitch e labs) Tau
      (s with bp := el i labs)) ∧
 
   (∀prog s v fname bname es t ret1 ret2 vals f.
@@ -450,7 +450,7 @@ Inductive step_term:
    list_rel (eval_exp s) es vals
    ⇒
    step_term prog s
-     (Call v (Lab_name fname bname) es t ret1 ret2)
+     (Call v (Lab_name fname bname) es t ret1 ret2) Tau
      <| bp := Lab_name fname bname;
         glob_addrs := s.glob_addrs;
         locals := alist_to_fmap (zip (f.params, vals));
@@ -466,7 +466,7 @@ Inductive step_term:
    s.stack = top::rest
    ⇒
    step_term prog s
-     (Return e)
+     (Return e) Tau
      <| bp := top.ret;
         glob_addrs := s.glob_addrs;
         locals := top.saved_locals |+ (top.ret_var, r);
@@ -476,7 +476,7 @@ Inductive step_term:
   (∀prog s e i size.
    eval_exp s e (FlatV (IntV i size))
    ⇒
-   step_term prog s (Exit e) (s with status := Complete i))
+   step_term prog s (Exit e) (Exit i) (s with status := Complete i))
   (* TODO Throw *)
 
 End
@@ -485,22 +485,26 @@ End
  * instruction pointer and do a big-step evaluation for each block *)
 Inductive step_block:
 
-  (∀prog s1 t s2.
-   step_term prog s1 t s2
+  (∀prog s1 t l s2.
+   step_term prog s1 t l s2
    ⇒
-   step_block prog s1 [] [] t s2) ∧
+   step_block prog s1 [] t [l] s2) ∧
 
-  (∀prog s1 i1 i2 l1 is t s2.
-   step_inst s1 i1 l1 s2 ∧
-   (¬?l2 s3. step_inst s2 i2 l2 s3)
+  (∀prog s1 t.
+   ¬(∃s2 (l:var obs). step_term prog s1 t l s2)
    ⇒
-   step_block prog s1 (i1::i2::is) [l1] t (s2 with status := Stuck)) ∧
+   step_block prog s1 [] t [Error] (s1 with status := Stuck)) ∧
+
+  (∀prog s1 i1 is t.
+   (¬∃l s2. step_inst s1 i1 l s2)
+   ⇒
+   step_block prog s1 (i1::is) t [Error] (s1 with status := Stuck)) ∧
 
   (∀prog s1 i l is ls t s2 s3.
    step_inst s1 i l s2 ∧
-   step_block prog s2 is ls t s3
+   step_block prog s2 is t ls s3
    ⇒
-   step_block prog s1 (i::is) (l::ls) t s3)
+   step_block prog s1 (i::is) t (l::ls) s3)
 
 End
 
@@ -516,7 +520,7 @@ End
 Inductive step:
   ∀prog s b ls s'.
     get_block prog s.bp b ∧
-    step_block prog s b.cmnd ls b.term s' ∧
+    step_block prog s b.cmnd b.term ls s' ∧
     s.status = Partial
     ⇒
     step prog s ls s'
